

ćwiczenia 1

October 27, 2021

1. (a) $7 + 4i + 3(5 - 9i) = 7 + 4i + 15 - 27i = 22 - 23i$
- (b) $Im(3 + 2i)(4 - 2i) - Re(5 + 3i)(1 - 4i) = 2(4 + 2i) - 5(1 - 4i) = 8 - 4i - 5 - 20 = 3 + 16i$
- (c) $(3 - 2i)(3 + 4i) = 9 + 12i - 6i - 8i^2 = 17 + 6i$
- (d) $(4 - 5i)(4 + 5i) = 4^2 - (5i)^2 = 16 + 25 = 41$
- (e) $\frac{-11+7i}{2+6i} = \frac{(-11+7i)(2-6i)}{(2+6i)(2-6i)} = \frac{-22+66i+14i-42i^2}{4+36} = \frac{20+80i}{40} = \frac{1}{2} + 2i$
- (f) $\frac{-1+2i}{5-3i} = \frac{(-1+2i)(5+3i)}{(5-3i)(5+3i)} = \frac{-5-3i+10i+6i^2}{25+9} = \frac{-11+7i}{31} = -\frac{11}{31} + \frac{7i}{31}$
- (g) $\frac{3+i}{2-5i} = \frac{(3+i)(2+5i)}{(2-5i)(2+5i)} = \frac{6+15i+2i+5i^2}{4+25} = \frac{1+17i}{29} = \frac{1}{29} + \frac{17i}{29}$
- (h) $\frac{5+3i}{8-2i} = \frac{(5+3i)(8+2i)}{(8-2i)(8+2i)} = \frac{40+10i+24i+6i^2}{64+4} = \frac{34+34i}{68} = \frac{1}{2} + \frac{1}{2}i$
- (i) $\frac{3+2i}{-1+3i} = \frac{(3+2i)(-1-3i)}{(-1+3i)(-1-3i)} = \frac{-3-9i-2i-6i^2}{1+9} = \frac{3-11i}{4} = \frac{3}{4} - \frac{11i}{4}$

2. (a)

$$5a - b = 5$$

$$-b - a = 4$$

$$a + b = -4$$

$$b = -4 - a$$

$$2z + (3 - i)\bar{z} = 5 + 4i$$

$$2(a + bi) + (3 - i)(a - bi) = 5 + 4i$$

$$2a + 2bi + 3a - 3bi - ai + bi^2 = 5 + 4i$$

$$5a - bi - ai - b = 5 + 4i$$

$$5a - b + i(-b - a) = 5 + 4i$$

$$5a - (-4 - a) = 5$$

$$5a + 4 + a = 5$$

$$6a = 1$$

$$a = \frac{1}{6}$$

$$b = -4 - \frac{1}{6}$$

$$b = -\frac{25}{6}$$

$$z = \frac{1}{6} - \frac{25}{6}i$$

(b)